tuned

PDS/PDS_Code.thy
@@ -8,13 +8,17 @@ global_interpretation pds: PDS_with_P_automata \<Delta> F_ctr_loc F_ctr_loc_st
   and F_ctr_loc_st :: "('state::finite) set"
   defines pre_star = "PDS_with_P_automata.pre_star_exec \<Delta>"
   and pre_star_check = "PDS_with_P_automata.pre_star_exec_check \<Delta>"
+  and initials = "PDS_with_P_automata.initials"
+  and finals = "PDS_with_P_automata.finals F_ctr_loc F_ctr_loc_st"
   and accepts = "PDS_with_P_automata.accepts F_ctr_loc F_ctr_loc_st"
+  and language = "PDS_with_P_automata.language F_ctr_loc F_ctr_loc_st"
+  and step_starp = "rtranclp (LTS.step_relp (PDS.transition_rel \<Delta>))"
   and accepts_pre_star_check = "PDS_with_P_automata.accept_pre_star_exec_check \<Delta> F_ctr_loc F_ctr_loc_st"
   .
 
 global_interpretation inter: Intersection_P_Automaton
-  initial_automaton "pds.finals initial_F_ctr_loc initial_F_ctr_loc_st" pds.initials
-  "pre_star \<Delta> final_automaton" "pds.finals final_F_ctr_loc final_F_ctr_loc_st"
+  initial_automaton "finals initial_F_ctr_loc initial_F_ctr_loc_st" initials
+  "pre_star \<Delta> final_automaton" "finals final_F_ctr_loc final_F_ctr_loc_st"
   for \<Delta> :: "('ctr_loc::{enum, linorder}, 'label::{finite, linorder}) rule set"
   and initial_automaton :: "(('ctr_loc, 'state::finite, 'label) state, 'label) transition set"
   and initial_F_ctr_loc :: "'ctr_loc set"
@@ -22,25 +26,25 @@ global_interpretation inter: Intersection_P_Automaton
   and final_automaton :: "(('ctr_loc, 'state, 'label) state, 'label) transition set"
   and final_F_ctr_loc :: "'ctr_loc set"
   and final_F_ctr_loc_st :: "'state set"
-  defines nonempty = "P_Automaton.nonempty
+  defines nonempty_inter = "P_Automaton.nonempty
     (inters initial_automaton (pre_star \<Delta> final_automaton))
-    (inters_finals (pds.finals initial_F_ctr_loc initial_F_ctr_loc_st)
-                   (pds.finals final_F_ctr_loc final_F_ctr_loc_st))
-    ((\<lambda>x. (x,x)) ` pds.initials)"
+    (inters_finals (finals initial_F_ctr_loc initial_F_ctr_loc_st)
+                   (finals final_F_ctr_loc final_F_ctr_loc_st))
+    ((\<lambda>x. (x,x)) ` initials)"
   .
 
 definition "check \<Delta> I IF IF_st F FF FF_st =
-  (if pds.initials \<subseteq> LTS.sources F then Some (nonempty \<Delta> I IF IF_st F FF FF_st) else None)"
+  (if pds.initials \<subseteq> LTS.sources F then Some (nonempty_inter \<Delta> I IF IF_st F FF FF_st) else None)"
 
-lemma check_None: "check \<Delta> I IF IF_st F FF FF_st = None \<longleftrightarrow> \<not> (pds.initials \<subseteq> LTS.sources F)"
+lemma check_None: "check \<Delta> I IF IF_st F FF FF_st = None \<longleftrightarrow> \<not> (initials \<subseteq> LTS.sources F)"
   unfolding check_def by auto
 
 lemma check_Some: "check \<Delta> I IF IF_st F FF FF_st = Some b \<longleftrightarrow>
-  (pds.initials \<subseteq> LTS.sources F \<and> b = (\<exists>p w p' w'.
-     (p, w) \<in> pds.language IF IF_st I \<and>
-     (p', w') \<in> pds.language FF FF_st F \<and>
-     pds.step_starp \<Delta> (p, w) (p', w')))"
-  unfolding check_def nonempty_def P_Automaton.nonempty_def
+  (initials \<subseteq> LTS.sources F \<and> b = (\<exists>p w p' w'.
+     (p, w) \<in> language IF IF_st I \<and>
+     (p', w') \<in> language FF FF_st F \<and>
+     step_starp \<Delta> (p, w) (p', w')))"
+  unfolding check_def nonempty_inter_def P_Automaton.nonempty_def
     inter.language_aut_alt inter.inters_language
     pds.language_aut_language
   by (auto 0 5 simp: pds.pre_star_exec_language_correct pds.pre_star_def image_iff
